src/Curve25519_Hop4.ec
@@ -80,7 +80,7 @@ qed.
 
 equiv eq_h4_add_sss : MHop2.add ~ M.__add4_sss:
    f{1} = inzpRep4 fs{2} /\
-   g{1} = inzpRep4 g{2}
+   g{1} = inzpRep4 gs{2}
     ==>
    res{1} = inzpRep4 res{2}.
 proof.
@@ -89,7 +89,7 @@ admit.
 qed.
 
 equiv eq_h4_add_rrs : MHop2.add ~ M.__add4_rrs:
-   f{1} = inzpRep4 fs{2} /\
+   f{1} = inzpRep4 f{2} /\
    g{1} = inzpRep4 g{2}
     ==>
    res{1} = inzpRep4 res{2}.
@@ -149,7 +149,7 @@ proc.
 admit.
 qed.
 
-equiv eq_h4_mul_pp : MHop2.mul ~ M.__mul4_pp:
+equiv eq_h4_mul_pp : MHop2.mul ~ M._mul4_pp:
    f{1} = inzpRep4 xa{2} /\
    g{1} = inzpRep4 ya{2}
     ==>
@@ -160,7 +160,7 @@ admit.
 qed.
 
 
-equiv eq_h4_mul_sss : MHop2.mul ~ M.__mul4_s_:
+equiv eq_h4_mul_ss : MHop2.mul ~ M._mul4_ss_:
    f{1} = inzpRep4 xa{2} /\
    g{1} = inzpRep4 ya{2}
     ==>
@@ -189,7 +189,7 @@ proc.
 admit.
 qed.
 
-equiv eq_h4_sqr_ss_ : MHop2.sqr ~ M.__sqr4_ss_:
+equiv eq_h4_sqr_ss_ : MHop2.sqr ~ M._sqr4_ss_:
     f{1} = inzpRep4 xa{2}
     ==>
     res{1} = inzpRep4 res{2}.
@@ -214,33 +214,33 @@ equiv eq_h4_tobytes :
 true ==> true.
 proof.
   admit.
-qed
+qed.
 
 equiv eq_h4_load :
-    MHop2.load ~ M.__load4:
+    MHop2.load ~ M.__load4 : 
 true ==> true.
 proof.
   admit.
-qed
+qed.
 
 equiv eq_h4_store :
-    MHop2.store ~ M.__store4:
+    MHop2.store ~ M.__store4 : 
 true ==> true.
 proof.
   admit.
-qed
+qed.
 
 equiv eq_init_point4 :
-    MHop2.init_points ~ M.__init_points4 :
+    MHop2.init_points ~ M.__init_points4 : 
 true ==> true.
-proof
+proof.
   admit.
 qed.
 
 
 (** step 1 : decode_scalar_25519 **)
 equiv eq_h4_decode_scalar_25519 :
-  MHop2.decode_scalar_25519 ~ M.__decode_scalar:
+  MHop2.decode_scalar ~ M.__decode_scalar:
   true ==> true.
 proof.
 admit.
@@ -321,7 +321,25 @@ equiv eq_h4_add_and_double :
   res{1}.`4 = inzpRep4 res{2}.`4.
 proof.
 proc => /=.
- admit.
+  call eq_h4_mul_rss.
+  call eq_h4_mul_sss.
+  call eq_h4_add_sss.
+  call eq_h4_sqr_ss.
+  call eq_h4_mul_a24_ss.
+  call eq_h4_sqr_ss.
+  call eq_h4_sub_sss.
+  call eq_h4_mul_sss.
+  call eq_h4_sub_sss.
+  call eq_h4_add_sss.
+  call eq_h4_sqr_ss.
+  call eq_h4_sqr_ss.
+  call eq_h4_mul_sss.
+  call eq_h4_mul_sss.
+  call eq_h4_add_sss.
+  call eq_h4_sub_sss.
+  call eq_h4_add_ssr.
+  call eq_h4_sub_ssr.
+  wp. done.
 qed.
 
 (** step 6 : montgomery_ladder_step **)
@@ -342,41 +360,20 @@ qed.
 
  (** step 8 : iterated square, may be error in variable names, ened to chec  **)
 equiv eq_h4_it_sqr :
- MHop2.it_sqr ~ M._it_sqr4_s_:
+ MHop2.it_sqr ~ M._it_sqr4_p:
    f{1}            =    inzpRep4 x{2} /\
    i{1}            =    to_uint i{2}  /\
-   i{1}            <=   W64.modulus   /\
+    i{1}           <=   W32.modulus   /\
     2              <=   i{1}          /\
    i{1} %% 2        =   0
    ==>
    res{1} = inzpRep4 res{2}.
 proof.
-  proc.
-(*
-  while (f{1}            =    inzpRep4 r{2}            /\ 
-         i{1}            =    to_uint i{2}             /\
-         i{1}            <=   W64.modulus              /\
-         0               <=   i{1}                     /\
-         i{1}            %%   2 = 0 /\
-         r{2} = (i{2} = W64.zero)).
-  swap 2 3 3. wp. conseq(_: _ ==> f{1} = inzpRep4 f{2}).
-  move=> &1 &2 [#] ????? ->> ?? ??? /=.
-    rewrite /DEC_64 /rflags_of_aluop_nocf64 /ZF_of_w64 => /=.
-    progress.
-    smt(@W64). move : H1; smt(). smt(). smt(). smt(@W64). smt(@W64).
-  by do 2! call eq_h4_sqr; skip; done.
-  swap 3 4 4. wp. conseq(_: _ ==> f{1} = inzpRep4 f{2}).
-  move=> &1 &2 [#] /= ->> ->> ??? ?? ->> /=.
-    rewrite /DEC_64 /rflags_of_aluop_nocf64 /ZF_of_w64 => /=.
-    progress.
-    smt(@W64). move : H1; smt(). smt(). smt(). smt(@W64). smt(@W64).
-  by do 2! call eq_h4_sqr; wp; skip; done.
-  *)
-admit.
+ admit.
 qed.
 
-equiv eq_h4_it_sqr_p :
- MHop2.it_sqr ~ M._it_sqr4_p:
+equiv eq_h4_it_sqr_s :
+ MHop2.it_sqr ~ M._it_sqr4_s_:
    f{1}            =    inzpRep4 x{2} /\
    i{1}            =    to_uint i{2}  /\
    i{1}            <=   W64.modulus   /\
@@ -408,7 +405,8 @@ equiv eq_h4_it_sqr_ss_ :
    ==>
    res{1} = inzpRep4 res{2}.
 proof.
-  proc.
+  proc. admit.
+qed.
 
 (** step 10 : encode point **)
 equiv eq_h4_encode_point : 
@@ -450,7 +448,7 @@ admit.
 qed.
 
 equiv eq_h4_scalarmult_base_ptr :
-  MHop2.scalarmult_base ~ M._curve25519_ref4_base_ptr:
+  MHop2.scalarmult_base ~ M.__curve25519_ref4_base_ptr:
   true ==> true.
 proof.
 admit.
@@ -458,14 +456,14 @@ qed.
 
 
 equiv eq_h4_scalarmult_jade :
-  MHop2.scalarmult_jade ~ M.jade_scalarmult_curve25519_amd64_ref4:
+  MHop2.scalarmult ~ M.jade_scalarmult_curve25519_amd64_ref4:
   true ==> true.
 proof.
 admit.
 qed.
 
 equiv eq_h4_scalarmult_jade_base :
-  MHop2.scalarmult_jade_base ~ M.jade_scalarmult_curve25519_amd64_ref4_base:
+  MHop2.scalarmult_base ~ M.jade_scalarmult_curve25519_amd64_ref4_base:
   true ==> true.
 proof.
 admit.
